# LV2 Port Groups Extension
# PROVISIONAL
# Copyright (C) 2009 Dave Robillard <dave@drobilla.net>
# Copyright (C) 2009 Lars Luthman <lars.luthman@gmail.com>
#
# Permission is hereby granted, free of charge, to any person obtaining a
# copy of this software and associated documentation files (the "Software"),
# to deal in the Software without restriction, including without limitation
# the rights to use, copy, modify, merge, publish, distribute, sublicense,
# and/or sell copies of the Software, and to permit persons to whom the
# Software is furnished to do so, subject to the following conditions:
# 
# The above copyright notice and this permission notice shall be included
# in all copies or substantial portions of the Software.
# 
# THE SOFTWARE IS PROVIDED "AS IS", WITHOUT WARRANTY OF ANY KIND, EXPRESS OR
# IMPLIED, INCLUDING BUT NOT LIMITED TO THE WARRANTIES OF MERCHANTABILITY,
# FITNESS FOR A PARTICULAR PURPOSE AND NONINFRINGEMENT. IN NO EVENT SHALL
# THE AUTHORS OR COPYRIGHT HOLDERS BE LIABLE FOR ANY CLAIM, DAMAGES OR
# OTHER LIABILITY, WHETHER IN AN ACTION OF CONTRACT, TORT OR OTHERWISE,
# ARISING FROM, OUT OF OR IN CONNECTION WITH THE SOFTWARE OR THE USE OR
# OTHER DEALINGS IN THE SOFTWARE.

@prefix pg:   <http://lv2plug.in/ns/dev/port-groups#> .
@prefix lv2:  <http://lv2plug.in/ns/lv2core#> .
@prefix rdf:  <http://www.w3.org/1999/02/22-rdf-syntax-ns#> .
@prefix rdfs: <http://www.w3.org/2000/01/rdf-schema#> .
@prefix owl:  <http://www.w3.org/2002/07/owl#> .
@prefix xsd:  <http://www.w3.org/2001/XMLSchema> .
@prefix doap: <http://usefulinc.com/ns/doap#> .
@prefix foaf: <http://xmlns.com/foaf/0.1/> .

<http://lv2plug.in/ns/dev/port-groups> a lv2:Specification ;
	doap:license <http://usefulinc.com/doap/licenses/mit> ;
	doap:name	"LV2 Port Groups" ;
	rdfs:comment "Defines semantic groupings of LV2 ports" ;
	doap:maintainer [
		a foaf:Person ;
		foaf:name	 "Lars Luthman" ;
		foaf:mbox     <mailto:lars.luthman@gmail.com>
	] , [
		a foaf:Person ;
		foaf:name	 "Dave Robillard" ;
		foaf:homepage <http://drobilla.net/> ;
		rdfs:seeAlso  <http://drobilla.net/drobilla.rdf>
	] .


## Core Classes / Properties

pg:Group a rdfs:Class ;
	rdfs:label   "LV2 Port Group" ;
	rdfs:subClassOf [ a owl:Restriction ;
		owl:onProperty lv2:symbol ;
		owl:hasValue   xsd:string ;
        rdfs:comment   """
A pg:Group MUST have at least one string lv2:symbol.  This symbol must be
unique according to the same rules as the lv2:symbol for an lv2:Port, where
group symbols and port symbols reside in the same namespace.  In other words,
a group on a plugin MUST NOT have the same symbol as another group or a port
on that plugin.  Rationale: Hosts or bindings may find it useful to construct
an identifier to refer to groups for the same reasons this is useful for ports.
"""
	] ;
	rdfs:comment """
A grouping of ports that can be logically considered a "stream", e.g.
two audio ports in a group forming a stereo stream.  Both inputs and outputs
can form a group, which allows describing to the host which outputs correspond
to which inputs.  In this case, outputs with a given role correspond to the
inputs in the same group with that role (though the output and input roles
of a group do not necessarily match).  The pg:source predicate can also be
used to describe this correspondence between separate ports/groups.
""" .

pg:requiredRole a rdf:Property ;
	rdfs:domain  pg:Group ;
	rdfs:range   lv2:Port ;
	rdfs:label   "Has port with role" ;
	rdfs:comment """
Indicates that a group always has a port with a particular role.
""" .

pg:optionalRole a rdf:Property ;
	rdfs:domain  pg:Group ;
	rdfs:range   lv2:Port ;
	rdfs:label   "May have port with role" ;
	rdfs:comment """
Indicates that a group MAY have a port with a particular role.
""" .

pg:sideChainOf a rdf:Property ;
	rdfs:domain  pg:Group , lv2:Port ;
	rdfs:range   pg:Group , lv2:Port ;
	rdfs:label   "Side-chain of" ;
	rdfs:comment """
Indicates that this port or group should be considered a "side chain" of
some other port or group.  The precise definition of "side chain" depends
on the plugin, but in general this group should be considered a modifier to
some other group, rather than an independent input itself.
""" .

pg:source a rdf:Property ;
	rdfs:domain  pg:Group , lv2:Port ;
	rdfs:range   pg:Group , lv2:Port ;
	rdfs:label   "Source group" ;
	rdfs:comment """
Indicates that this port or group should be considered the "result" of
some other port or group.  This property only makes sense on groups with
outputs when the source is a group with inputs.  This can be used to convey
a relationship between corresponding input and output groups with different
types, e.g.  a mono->stereo plugin.
""" .

pg:encodedType a rdf:Property ;
	rdfs:domain  pg:Group ;
	rdfs:range   rdfs:Class ;
	rdfs:label   "Is an encoding of" ;
	rdfs:comment """
Indicates this group is an encoding of some other group type, e.g. 4.0
encoded in 2.0 would be a StereoGroup with pg:encodedType FourPointZeroGroup.
""" .

pg:mainGroup a rdf:Property ;
	rdfs:domain  lv2:Plugin ;
	rdfs:range   pg:Group ;
	rdfs:label   "Main port group" ;
	rdfs:comment """
Indicates that this group should be considered the "main" inputs/outputs of
the plugin, e.g. it probably makes sense to just connect main groups and set
some controls.  A plugin MUST NOT have more than one :mainGroup property.
High-level hosts that simply want to insert an plugin in a given stream
should use this property to determine where the plugin 'fits'.
""" .

pg:inGroup a rdf:Property ;
	rdfs:domain  lv2:Port ;
	rdfs:range   pg:Group ;
	rdfs:label   "In port group" ;
	rdfs:comment """
Indicates that this port is a part of a group of ports on the plugin.
Ports that have a meaningful "role" that may be useful to hosts SHOULD also
have a :role property, otherwise ports in the group have no meaningful order.
""" .

pg:Role a rdfs:Class ;
	rdfs:label   "Port role" ;
	rdfs:comment """
The role of a port with respect to its plugin or group.  If the port is a
member of a group (has an :inGroup property) the role is relevant with respect
to that group.  Otherwise the role is relevant with respect to the plugin.
""" .

pg:hasRole a rdf:Property ;
	rdfs:domain  lv2:Port ;
	rdfs:range   pg:Role ;
	rdfs:label   "Has role" ;
	rdfs:comment """
Indicates that this port has a particular role with respect to its enclosing
plugin or group (whichever is smaller).  A port may have several roles if it
makes sense to do so (though some Role or Group definition may forbid this).
""" .


## Standard Roles

pg:leftChannel          a pg:Role ; rdfs:label "Left" .
pg:rightChannel         a pg:Role ; rdfs:label "Right" .
pg:centerChannel        a pg:Role ; rdfs:label "Center" .
pg:sideChannel          a pg:Role ; rdfs:label "Side" .
pg:surroundChannel      a pg:Role ; rdfs:label "Surround" .
pg:leftSurroundChannel  a pg:Role ; rdfs:label "Left Surround" .
pg:rightSurroundChannel a pg:Role ; rdfs:label "Right Surround" .
pg:leftRearChannel      a pg:Role ; rdfs:label "Left Rear" .
pg:rightRearChannel     a pg:Role ; rdfs:label "Right Rear" .
pg:subChannel           a pg:Role ; rdfs:label "Sub (LFE)" .
pg:amplitude            a pg:Role ; rdfs:label "Amplitude" .
pg:attack               a pg:Role ; rdfs:label "Attach" .
pg:cutoffFrequency      a pg:Role ; rdfs:label "Cutoff Frequency" .
pg:decay                a pg:Role ; rdfs:label "Decay" .
pg:delay                a pg:Role ; rdfs:label "Delay" .
pg:frequency            a pg:Role ; rdfs:label "Frequency" .
pg:hold                 a pg:Role ; rdfs:label "Hold" .
pg:pulseWidth           a pg:Role ; rdfs:label "Pulse Width" .
pg:ratio                a pg:Role ; rdfs:label "Ratio" .
pg:release              a pg:Role ; rdfs:label "Release" .
pg:resonance            a pg:Role ; rdfs:label "Resonance" .
pg:sustain              a pg:Role ; rdfs:label "Sustain" .
pg:threshold            a pg:Role ; rdfs:label "Threshold" .
pg:waveform             a pg:Role ; rdfs:label "Waveform" .


## Standard Groups 

pg:MonoGroup a pg:Group ;
	rdfs:label "Mono" ;
	pg:hasPort pg:centerChannel .

pg:StereoGroup a pg:Group ;
	rdfs:label "Stereo" ;
	pg:hasPort pg:leftChannel ;
	pg:hasPort pg:rightChannel .

pg:MidSideGroup a pg:Group ;
	rdfs:label "Mid-Side Stereo" ;
	pg:hasPort pg:centerChannel ;
	pg:hasPort pg:sideChannel .

pg:ThreePointZeroGroup a pg:Group ;
	rdfs:label "3.0 Surround" ;
	pg:hasPort pg:leftChannel ;
	pg:hasPort pg:rightChannel ;
	pg:hasPort pg:surroundChannel .

pg:FourPointZeroGroup a pg:Group ;
	rdfs:label "4.0 Surround (Quadraphonic)" ;
	pg:hasPort pg:leftChannel ;
	pg:hasPort pg:rightChannel ;
	pg:hasPort pg:centerChannel ;
	pg:hasPort pg:surroundChannel .

pg:FivePointZeroGroup a pg:Group ;
	rdfs:label "5.0 Surround (3-2 stereo)" ;
	pg:hasPort pg:leftChannel ;
	pg:hasPort pg:rightChannel ;
	pg:hasPort pg:centerChannel ;
	pg:hasPort pg:leftSurroundChannel ;
	pg:hasPort pg:rightSurroundChannel .

pg:FivePointOneGroup a pg:Group ;
	rdfs:label "5.1 Surround (3-2 stereo)" ;
	pg:hasPort pg:leftChannel ;
	pg:hasPort pg:rightChannel ;
	pg:hasPort pg:centerChannel ;
	pg:hasPort pg:leftSurroundChannel ;
	pg:hasPort pg:rightSurroundChannel ;
	pg:hasPort pg:lfeChannel .

pg:SixPointOneGroup a pg:Group ;
	rdfs:label "6.1 Surround" ;
	pg:hasPort pg:leftChannel ;
	pg:hasPort pg:rightChannel ;
	pg:hasPort pg:centerChannel ;
	pg:hasPort pg:leftSurroundChannel ;
	pg:hasPort pg:rightSurroundChannel ;
	pg:hasPort pg:centerRearChannel ;
	pg:hasPort pg:lfeChannel .

pg:SevenPointOneGroup a pg:Group ;
	rdfs:label "7.1 Surround" ;
	pg:hasPort pg:leftChannel ;
	pg:hasPort pg:rightChannel ;
	pg:hasPort pg:centerChannel ;
	pg:hasPort pg:leftSurroundChannel ;
	pg:hasPort pg:rightSurroundChannel ;
	pg:hasPort pg:leftRearChannel ;
	pg:hasPort pg:rightRearChannel ;
	pg:hasPort pg:lfeChannel .

pg:AmbisonicBH1V0Group a pg:Group ;
	rdfs:label "Ambisonic B stream of horizontal order 1 and vertical order 0." ;
	pg:hasPort pg:wChannel ;
	pg:hasPort pg:xChannel ;
	pg:hasPort pg:yChannel .

pg:AmbisonicBH1V1Group a pg:Group ;
	rdfs:label "Ambisonic B stream of horizontal order 1 and vertical order 1." ;
	pg:hasPort pg:wChannel ;
	pg:hasPort pg:xChannel ;
	pg:hasPort pg:yChannel ;
	pg:hasPort pg:zChannel .

pg:AmbisonicBH2V0Group a pg:Group ;
	rdfs:label "Ambisonic B stream of horizontal order 2 and vertical order 0." ;
	pg:hasPort pg:wChannel ;
	pg:hasPort pg:xChannel ;
	pg:hasPort pg:yChannel ;
	pg:hasPort pg:uChannel ;
	pg:hasPort pg:vChannel .

pg:AmbisonicBH2V1Group a pg:Group ;
	rdfs:label "Ambisonic B stream of horizontal order 2 and vertical order 1." ;
	pg:hasPort pg:wChannel ;
	pg:hasPort pg:xChannel ;
	pg:hasPort pg:yChannel ;
	pg:hasPort pg:zChannel ;
	pg:hasPort pg:uChannel ;
	pg:hasPort pg:vChannel .

pg:AmbisonicBH2V2Group a pg:Group ;
	rdfs:label "Ambisonic B stream of horizontal order 2 and vertical order 2." ;
	pg:hasPort pg:wChannel ;
	pg:hasPort pg:xChannel ;
	pg:hasPort pg:yChannel ;
	pg:hasPort pg:zChannel ;
	pg:hasPort pg:rChannel ;
	pg:hasPort pg:sChannel ;
	pg:hasPort pg:tChannel ;
	pg:hasPort pg:uChannel ;
	pg:hasPort pg:vChannel .

pg:AmbisonicBH3V0Group a pg:Group ;
	rdfs:label "Ambisonic B stream of horizontal order 3 and vertical order 0." ;
	pg:hasPort pg:wChannel ;
	pg:hasPort pg:xChannel ;
	pg:hasPort pg:yChannel ;
	pg:hasPort pg:uChannel ;
	pg:hasPort pg:vChannel ;
	pg:hasPort pg:pChannel ;
	pg:hasPort pg:qChannel .

pg:AmbisonicBH3V1Group a pg:Group ;
	rdfs:label "Ambisonic B stream of horizontal order 3 and vertical order 1." ;
	pg:hasPort pg:wChannel ;
	pg:hasPort pg:xChannel ;
	pg:hasPort pg:yChannel ;
	pg:hasPort pg:zChannel ;
	pg:hasPort pg:uChannel ;
	pg:hasPort pg:vChannel ;
	pg:hasPort pg:pChannel ;
	pg:hasPort pg:qChannel .

pg:AmbisonicBH3V2Group a pg:Group ;
	rdfs:label "Ambisonic B stream of horizontal order 3 and vertical order 2." ;
	pg:hasPort pg:wChannel ;
	pg:hasPort pg:xChannel ;
	pg:hasPort pg:yChannel ;
	pg:hasPort pg:zChannel ;
	pg:hasPort pg:rChannel ;
	pg:hasPort pg:sChannel ;
	pg:hasPort pg:tChannel ;
	pg:hasPort pg:uChannel ;
	pg:hasPort pg:vChannel ;
	pg:hasPort pg:pChannel ;
	pg:hasPort pg:qChannel .

pg:AmbisonicBH3V3Group a pg:Group ;
	rdfs:label "Ambisonic B stream of horizontal order 3 and vertical order 3." ;
	pg:hasPort pg:wChannel ;
	pg:hasPort pg:xChannel ;
	pg:hasPort pg:yChannel ;
	pg:hasPort pg:zChannel ;
	pg:hasPort pg:rChannel ;
	pg:hasPort pg:sChannel ;
	pg:hasPort pg:tChannel ;
	pg:hasPort pg:uChannel ;
	pg:hasPort pg:vChannel ;
	pg:hasPort pg:kChannel ;
	pg:hasPort pg:lChannel ;
	pg:hasPort pg:mChannel ;
	pg:hasPort pg:nChannel ;
	pg:hasPort pg:oChannel ;
	pg:hasPort pg:pChannel ;
	pg:hasPort pg:qChannel .

pg:EnvelopeControlGroup a pg:Group ;
	rdfs:label "The controls for an envelope." ;
	pg:mayHavePort pg:delay ;
	pg:mayHavePort pg:attack ;
	pg:mayHavePort pg:hold ;
	pg:mayHavePort pg:decay ;
	pg:mayHavePort pg:sustain ;
	pg:mayHavePort pg:release .

pg:OscillatorControlGroup a pg:Group ;
	rdfs:label "The controls for an oscillator." ;
	pg:mayHavePort pg:frequency ;
	pg:mayHavePort pg:amplitude ;
	pg:mayHavePort pg:waveform ;
	pg:mayHavePort pg:pulseWidth .

pg:FilterControlGroup
	rdfs:label "The controls for a filter." ;
	pg:mayHavePort pg:cutoffFrequency ;
	pg:mayHavePort pg:resonance .

pg:CompressorControlGroup
	rdfs:label "The controls for a compressor." ;
	pg:mayHavePort pg:threshold ;
	pg:mayHavePort pg:ratio .

