# LV2 Port Groups Extension
# PROVISIONAL
# Copyright (C) 2009 Dave Robillard <dave@drobilla.net>
#
# Permission is hereby granted, free of charge, to any person obtaining a
# copy of this software and associated documentation files (the "Software"),
# to deal in the Software without restriction, including without limitation
# the rights to use, copy, modify, merge, publish, distribute, sublicense,
# and/or sell copies of the Software, and to permit persons to whom the
# Software is furnished to do so, subject to the following conditions:
# 
# The above copyright notice and this permission notice shall be included
# in all copies or substantial portions of the Software.
# 
# THE SOFTWARE IS PROVIDED "AS IS", WITHOUT WARRANTY OF ANY KIND, EXPRESS OR
# IMPLIED, INCLUDING BUT NOT LIMITED TO THE WARRANTIES OF MERCHANTABILITY,
# FITNESS FOR A PARTICULAR PURPOSE AND NONINFRINGEMENT. IN NO EVENT SHALL
# THE AUTHORS OR COPYRIGHT HOLDERS BE LIABLE FOR ANY CLAIM, DAMAGES OR
# OTHER LIABILITY, WHETHER IN AN ACTION OF CONTRACT, TORT OR OTHERWISE,
# ARISING FROM, OUT OF OR IN CONNECTION WITH THE SOFTWARE OR THE USE OR
# OTHER DEALINGS IN THE SOFTWARE.

@prefix :     <http://lv2plug.in/ns/dev/port-groups#> .
@prefix lv2:  <http://lv2plug.in/ns/lv2core#> .
@prefix rdf:  <http://www.w3.org/1999/02/22-rdf-syntax-ns#> .
@prefix rdfs: <http://www.w3.org/2000/01/rdf-schema#> .
@prefix owl:  <http://www.w3.org/2002/07/owl#> .
@prefix xsd:  <http://www.w3.org/2001/XMLSchema> .
@prefix doap: <http://usefulinc.com/ns/doap#> .
@prefix foaf: <http://xmlns.com/foaf/0.1/> .

<http://lv2plug.in/ns/dev/port-groups> a lv2:Specification ;
	doap:license <http://usefulinc.com/doap/licenses/mit> ;
	doap:name    "LV2 Port Groups" ;
	rdfs:comment "Defines groupings of LV2 ports into multi-channel streams" ;
	doap:maintainer [
		a foaf:Person ;
		foaf:name     "Dave Robillard" ;
		foaf:homepage <http://drobilla.net/> ;
		rdfs:seeAlso  <http://drobilla.net/drobilla.rdf>
	] .


## Core Classes / Properties

:Group a rdfs:Class ;
    rdfs:label   "LV2 Port Group" ;
    rdfs:comment """
A grouping of ports that can be logically considered a "stream", e.g.
two audio ports in a group forming a stereo stream.  Both inputs and
outputs can form a group, which allows describing to the host which
outputs correspond to which inputs.  In this case, outputs with a given
role correspond to the inputs in the same group with that role (though
the output and input roles of a group do not necessarily match).
""" .

:mainGroup a rdf:Property ;
	rdfs:domain  lv2:Plugin ;
	rdfs:range   :Group ;
    rdfs:label   "Main port group" ;
    rdfs:comment """
Indicates that this port group should be considered the "main" inputs/outputs
of the plugin, e.g. a stereo effect has a "main" group with 2 inputs and 2
outputs.  A plugin MUST have at most one :mainGroup property.
""" .

:inGroup a rdf:Property ;
	rdfs:domain  lv2:Port ;
	rdfs:range   :Group ;
    rdfs:label   "In port group" ;
    rdfs:comment """
Indicates that this port is a part of a group of ports on the plugin.
Ports that have a meaningful "role" that may be useful to hosts SHOULD
also have a :role property, otherwise ports in the group have no meaningful
order.""" .

:Role a rdfs:Class ;
    rdfs:label   "Port role" ;
    rdfs:comment """
The role of a port with respect to its plugin or group.

If the port is a member of a group (has an :inGroup property) the
role is relevant with respect to that group.  Otherwise the role
is relevant with respect to the plugin.
""" .

:hasRole a rdf:Property ;
	rdfs:domain  lv2:Port ;
	rdfs:range   :Role ;
    rdfs:label   "Has role" ;
    rdfs:comment """
Indicates that this port has a particular role with respect to its enclosing
plugin or group (whichever is smaller).  A port may have several roles if it
makes sense to do so; some roles may forbid this or define more specific
restrictions.
""" .


## Standard Roles
#
# These can be used to describe stereo, 3.0, 4.0, 5.1, 6.1, 7.1, and more.

:left a :Role ;
	rdfs:label "Left" ;
	rdfs:comment "A port with this role MUST NOT also have the role :right" .

:right a :Role ;
	rdfs:label "Right" ;
	rdfs:comment "A port with this role MUST NOT also have the role :left" .

:center a :Role ;
	rdfs:label "Center" ;
	rdfs:comment """
The 'center' along the :left to :right axis.
Alone, it indicates the port is in the exact center of :left and :right.
It may also be combined with :left or :right to describe positions in-between,
describing 5 positions along the :left to :right axis:

 left (L), center-left (CL), center (C), center-right (CR), right (R)
""" .

:front a :Role ;
	rdfs:label "Front" ;
	rdfs:comment "A port with this role MUST NOT also have the role :back" .

:back a :Role ;
	rdfs:label "Back" ;
	rdfs:comment "A port with this role MUST NOT also have the role :front" .

:side a :Role ;
	rdfs:label "Side" ;
	rdfs:comment """
The 'center' along the :front to :back axis.
This may be combined with :front to :back in the same way :center may be
combined with :left and :right, though no common audio setups require this.
""" .

:sub a :Role ;
	rdfs:label "Sub" ;
	rdfs:comment """
A subwoofer, or "low frequency effects" (LFE) channel.
This role may be associated with a position using other roles,
but is usually used alone to designate a non-positional sub channel.
""" .


## Standard Groups 
#
# Plugins may either use these groups directly, or define their own groups
# which MAY be rdfs:subClassOf these groups.  If a group is a subclass of
# another group G, it must have at least the ports required by G, and any
# other ports in the group MUST be lv2:connectionOptional.

:Mono a :Group ;
	rdfs:label "Mono" ;
	rdfs:comment """A group with:
 * 1 :center
""" .

:Stereo a :Group ;
	rdfs:label "Stereo" ;
	rdfs:comment """A group with:
 * 1 :left
 * 1 :right
""" .

:FourPointZero a :Group ;
	rdfs:label "4.0 Surround" ;
	rdfs:comment """4.0 Surround (Quadraphonic), a group with:
 * 1 :front :left
 * 1 :front :right
 * 1 :rear  :left
 * 1 :rear  :right
""" .

:FivePointOne a :Group ;
	rdfs:label "5.1 Surround" ;
	rdfs:comment """5.1 Surround (3-2 stereo), a group with:
 * 1 :front :left
 * 1 :front :right
 * 1 :front :center (:front may be omitted)
 * 1 :rear  :left
 * 1 :rear  :right
 * 1 :sub
""" .

:SixPointOne a :Group ;
	rdfs:label "6.1 Surround" ;
	rdfs:comment """6.1 Surround, a group with:
 * 1 :front :left
 * 1 :front :right
 * 1 :front :center
 * 1 :side  :left
 * 1 :side  :right
 * 1 :rear  :center
 * 1 :sub
""" .

:SevenPointOne a :Group ;
	rdfs:label "7.1 Surround" ;
	rdfs:comment """7.1 Surround, a group with:
 * 1 :front :left
 * 1 :front :right
 * 1 :front :center
 * 1 :side  :left
 * 1 :side  :right
 * 1 :rear  :left
 * 1 :rear  :right
 * 1 :sub
""" .

:SevenPointOneWide a :Group ;
	rdfs:label "7.1 Surround (Wide)" ;
	rdfs:comment """7.1 Surround (Wide), a group with:
 * 1 :front :left
 * 1 :front :left :center
 * 1 :front :center
 * 1 :front :right :center
 * 1 :front :right
 * 1 :rear  :left
 * 1 :rear  :right
 * 1 :sub
""" .


